wasm: Redo wrap_result

compiler/backend/semantics/wasmSemScript.sml
@@ -72,11 +72,16 @@ val evaluate_nomatch_eq_none = Q.store_thm("evaluate_nomatch_eq_none[simp]",
   simp[evaluate_nomatch_def]
 )
 
-val wrap_result = Define `
-wrap_result l = case LENGTH l of
-                  | 0 => Result NONE
-                  | 1 => Result (SOME (HD l))
-                  | _ => TypeError "Expected result of at most one value"`
+val wrap_result_def = Define `
+  wrap_result l = if LENGTH l <= 1
+                  then Result (oHD l)
+                  else TypeError "Expected result of at most one value"
+`
+
+val wrap_result_eq_result = Q.store_thm("wrap_result_eq_result[simp]",
+  `LENGTH l < 2 ==> wrap_result l = Result (oHD l)`,
+  rw [wrap_result_def]
+)
 
 (* NOTE: We assume that any host function corresponding to a
  * foreign functionis of type [i32] ^ 4 -> []. *)
